proofs/core/Task.v
@@ -1,0 +1,183 @@
+Require Export FullInterp.
+Set Bullet Behavior "Strict Subproofs".
+
+(*A why3 task consists of
+   1. A context gamma (of abstract and concrete type, function, and
+    predicate defs)
+  2. A local context Delta of well-typed formulas
+  3. A local context of variables
+  4. A well-typed formula (the goal).
+  We defer the well-typed checks to a separate definition
+  so we can define transformations purely
+  syntactically *)
+
+Record task (gamma: context) : Set :=
+  mk_task {task_delta: list formula;
+    task_vars: list vsymbol;
+    task_goal: formula}.
+
+Arguments task_delta { _ }.
+Arguments task_vars { _ }.
+Arguments task_goal { _ }.
+
+(*We make this a record so we can refer to the hypotheses by name*)
+Record task_wf {gamma: context} (w: task gamma) :=
+  mk_task_wf
+  (*Context is well-typed*)
+  {task_gamma_valid: valid_context gamma;
+  (*Local context is well-typed*)
+  task_delta_typed: Forall (formula_typed gamma) (task_delta w);
+  (*All free vars in var list*)
+  task_delta_fv: Forall (fun f => sublist (fmla_fv f) (task_vars w)) (task_delta w);
+  (*All variable types are valid*)
+  task_vars_valid: Forall (fun x => valid_type gamma (snd x)) (task_vars w);
+  (*goal is well-typed*)
+  task_goal_typed: formula_typed gamma (task_goal w);
+  (*All free vars in goal in var list*)
+  task_goal_fv: sublist (fmla_fv (task_goal w)) (task_vars w)}.
+
+Arguments task_gamma_valid {_} {_}.
+Arguments task_delta_typed {_} {_}.
+Arguments task_delta_fv {_} {_}.
+Arguments task_vars_valid {_} {_}.
+Arguments task_goal_typed {_} {_}.
+Arguments task_goal_fv {_} {_}.
+
+(*A task is valid if delta |= f. But these formulas are closed,
+  so we write it a bit differently*)
+Definition task_valid (gamma: context) (w: task gamma)
+  (w_wf: task_wf w) : Prop :=
+  forall (pd: pi_dom) (pf: pi_funpred (task_gamma_valid w_wf) pd) (vt: val_typevar)
+    (vv: val_vars pd vt),
+    full_interp (task_gamma_valid w_wf) pd pf ->
+    (forall (f: formula) (f_in: In f (task_delta w)),
+      formula_rep (task_gamma_valid w_wf) 
+      pd vt pf vv f (Forall_In (task_delta_typed w_wf) f_in)) ->
+    formula_rep (task_gamma_valid w_wf) pd vt pf vv (task_goal w) 
+      (task_goal_typed w_wf).
+
+(*What this means: gamma, delta, vars |= f iff
+  gamma |= forall vars, delta -> f*)
+
+Lemma task_alt_typed (gamma: context) (w:task gamma)
+(w_wf: task_wf w):
+formula_typed gamma 
+(fforalls (task_vars w) (Fbinop Timplies (iter_fand (task_delta w)) (task_goal w))).
+Proof.
+  apply fforalls_valid.
+  - constructor.
+    + apply iter_fand_valid. apply w_wf.
+    + apply w_wf.
+  - apply w_wf.
+Qed.
+
+Fixpoint triv_var_hlist {pd: pi_dom} {vt: val_typevar}
+  (vv: val_vars pd vt) (vs: list vsymbol) :
+  hlist (fun x => domain (dom_aux pd) (v_subst vt x)) (map snd vs) :=
+  match vs as l return
+  hlist (fun x => domain (dom_aux pd) (v_subst vt x)) (map snd l) with
+  | nil => HL_nil _
+  | h :: t => HL_cons _ _ (map snd t) (vv h) (triv_var_hlist vv t)
+  end.
+
+Lemma substi_mult_base {pd vt} (v1 v2: val_vars pd vt) vs h x:
+  (forall x, v1 x = v2 x) ->
+  substi_mult pd vt v1 vs h x = substi_mult pd vt v2 vs h x.
+Proof.
+  revert v1 v2.
+  induction vs; simpl; auto.
+  intros. apply IHvs. intros.
+  unfold substi.
+  destruct (vsymbol_eq_dec x0 a); auto.
+Qed.
+  
+Lemma triv_var_hlist_substi pd vt vv vs:
+  forall x, substi_mult pd vt vv vs (triv_var_hlist vv vs) x =
+    vv x.
+Proof.
+  revert vv.
+  induction vs; simpl; auto.
+  intros.
+  rewrite substi_mult_base with(v2:=vv); auto.
+  intros. unfold substi. destruct (vsymbol_eq_dec x0 a); auto.
+  subst. reflexivity.
+Qed. 
+
+(*The theorem we want*)
+Theorem task_valid_equiv (gamma: context) (w:task gamma)
+  (w_wf: task_wf w) :
+  task_valid gamma w w_wf <->
+  valid (task_gamma_valid w_wf) (fforalls (task_vars w) 
+    (Fbinop Timplies (iter_fand (task_delta w)) (task_goal w)))
+  (task_alt_typed gamma w w_wf).
+Proof.
+  unfold valid, task_valid.
+  unfold satisfies. split; intros.
+  - erewrite fmla_rep_irrel.
+    rewrite fforalls_val.
+    rewrite simpl_all_dec.
+    intros h.
+    Unshelve.
+    2: {
+      constructor.
+      apply iter_fand_valid.
+      all: apply w_wf.
+    }
+    2: apply w_wf.
+    simpl.
+    simpl_rep_full.
+    rewrite bool_of_binop_impl, simpl_all_dec.
+    rewrite iter_fand_rep.
+    intros Hall.
+    erewrite fmla_rep_irrel.
+    apply H; auto.
+  - specialize (H pd pf H0).
+    unfold satisfies in H.
+    specialize (H vt vv).
+    erewrite fmla_rep_irrel in H.
+    erewrite fforalls_val in H.
+    rewrite simpl_all_dec in H.
+    (*We have to choose an hlist such that (substi_mult)
+      agrees with vv on all vars*)
+    specialize (H (triv_var_hlist vv (task_vars w))).
+    rewrite fmla_change_vv with(v2:=vv) in H.
+    2: {
+      intros. apply triv_var_hlist_substi.
+    }
+    revert H; simpl_rep_full;
+    rewrite bool_of_binop_impl, simpl_all_dec; intros.
+    erewrite fmla_rep_irrel. apply H.
+    rewrite iter_fand_rep. intros.
+    erewrite fmla_rep_irrel; apply H1.
+    Unshelve.
+    + constructor; try apply w_wf. apply iter_fand_valid, w_wf.
+    + apply w_wf.
+    + auto.
+Qed.
+
+(*Now we define a task transformation: a function that
+  produces 0 or more tasks from a task - called "tlist" in why3*)
+Definition trans (gamma: context) := task gamma -> list (task gamma).
+
+(*What does it mean for a transformation to be sound?
+  1. All resulting tasks are well-formed
+  2. If all resulting tasks are valid, then so is the original task*)
+
+(*The definition is a little awkward because of the double wf proof,
+  but it makes it easier to use*)
+Definition sound_trans {gamma: context} (T: trans gamma) : Prop :=
+  forall (t: task gamma) (t_wf: task_wf t),
+    Forall task_wf (T t) /\
+    ((forall (tr: task gamma) (tr_wf: task_wf tr), In tr (T t) ->
+      task_valid gamma tr tr_wf) ->
+    task_valid gamma t t_wf).
+
+(*As a trivial example, the identity transformation is sound*)
+Definition trans_id (gamma: context) : trans gamma := fun x => [x].
+
+Lemma sound_trans_id (gamma: context) : sound_trans (trans_id gamma).
+Proof.
+  unfold sound_trans. intros. split.
+  - unfold trans_id. constructor; auto.
+  - intros. apply H. simpl. auto.
+Qed.
